commentaires sur les eliminateurs et le tracage de list_args

aux_fun_tests.v
@@ -4,17 +4,118 @@ Add Rec LoadPath "/home/pierre/depots/sniper" as Sniper.
 Require Import utilities. 
 Require Import interpretation_algebraic_types.
 Require Import elimination_polymorphism.
+Require Import eliminators.
 Require Import MetaCoq.Template.All.
 Require Import String.
 Require Import List.
 Require Import ZArith.
 
-
+(* function to comment :  pose_inductive_tac *)
 
 Open Scope string_scope.  
 
 Import ListNotations MonadNotation. 
 
+
+
+Definition get_ind_ident (kerna : kername) := let (mdp , idind) := kerna in idind.
+
+
+Locate pose_inductive_tac.
+
+MetaCoq Quote Definition Type_reif := Eval hnf in Type.
+MetaCoq Quote Definition Prop_reif := Eval hnf in Prop.
+MetaCoq Quote Definition Set_reif := Eval hnf in Set.
+MetaCoq Quote Definition eq_reif := Eval hnf in @eq. 
+
+MetaCoq Quote Definition nat_reif := nat.
+MetaCoq Quote Recursively Definition nat_env_reif := nat.
+
+
+Definition list_nat := @list nat.
+MetaCoq Quote Definition list_nat_reif :=  (@list nat).
+MetaCoq Quote Recursively Definition list_nat_env_reif := list_nat.             
+MetaCoq Quote Definition cons_nat_type_reif := (nat -> list_nat -> list_nat).
+MetaCoq Quote Definition nil_type_reif := (forall (A : Type), list A).
+(* \Q nil_type_reif and cons_nat_reif do not work because do not
+currently have  the right universes levels *)
+
+
+MetaCoq Quote Definition cons_reif := cons.
+
+MetaCoq Quote Definition zero_reif := 0.
+MetaCoq Quote Definition one_reif := 1.
+MetaCoq Quote Definition two_reif := 2.
+
+
+MetaCoq Quote Definition nil_nat_reif := Eval cbn in (@nil nat).
+MetaCoq Quote Definition list_one_two_reif := Eval cbn in [1 ; 2].
+MetaCoq Quote Definition list_one_two_two_reif := Eval cbn in [1 ; 2 ; 2].
+
+MetaCoq Quote Definition list_one_two_two_reif' := (List.app [1] [2 ; 2]).
+
+
+
+(** Reified objects functions *)
+ 
+Definition cons_nat := @cons nat.
+
+
+
+MetaCoq Quote Definition length_reif := @List.length.
+MetaCoq Quote Definition le_reif := le.
+MetaCoq Quote Definition S_reif := Eval cbn in S.
+MetaCoq Quote Recursively Definition S_env_reif := S.
+Print S_env_reif.
+Print S_reif. 
+MetaCoq Quote Definition O_reif := O.
+MetaCoq Quote Definition add_reif := Eval cbn in Nat.add.
+MetaCoq Quote Definition nil_reif := nil.
+MetaCoq Quote Recursively Definition nil_env_reif := nil.
+MetaCoq Quote Recursively Definition cons_env_reif := cons.
+MetaCoq Quote Recursively Definition cons_nat_env_reif := cons_nat.
+MetaCoq Quote Definition cons_nat_reif := cons_nat.
+MetaCoq Quote Definition list_reif := @list.
+MetaCoq Quote Recursively Definition list_env_reif := @list.
+
+Print list_env_reif.
+
+Definition nat_indu := ltac:(let s := fresh in  pose_inductive_tac nat s ; exact s).
+Definition list_indu := ltac:(let s := fresh in  pose_inductive_tac list s ; exact s).
+Definition list_nat_indu := ltac:(let s := fresh in  pose_inductive_tac list s ; exact s).
+
+
+
+
+
+
+Definition nat_oind := {|
+ind_name := "nat"%string;
+ind_type := tSort (Universe.of_levels (inr Level.lSet));
+ind_kelim := IntoAny;
+ind_ctors := [("O"%string, tRel 0, 0);
+             ("S"%string,
+             tProd
+               {|
+               binder_name := nAnon;
+               binder_relevance := Relevant |}
+               (tRel 0) (tRel 1), 1)];
+ind_projs := [];
+ind_relevance := Relevant |}.
+
+
+
+Ltac pose_oind_tac t i idn := let s := fresh "s" in pose_mind_tac t s ; pose (nth i s.(ind_bodies)  nat_oind) as idn; simpl in idn ; clear s.
+(* pose_oind take an (unreified) inductive  I and outputs the i-th one_inductive_block of I *) 
+(* when I is not a mutual inductive, i should be equal to 0 *)
+(* the tactic uses nat_oind as the defaut value for nth *)
+
+Definition list_oind := ltac:(let s := fresh in pose_oind_tac list 0 s ; compute in s ; exact s).
+Print list_oind.
+
+ 
+
+(* 
 Inductive my_type :=
   | A : my_type
   | B : my_type -> my_type
@@ -24,6 +125,63 @@ MetaCoq Quote Definition mt_reif := my_type.
 MetaCoq Quote Definition A_reif := A. 
 MetaCoq Quote Definition B_reif := B.
 MetaCoq Quote Definition C_reif := C.
+*)
 
 
+(**** eliminators.v ****)
 
+Goal False.
+
+Print nil_type_reif.
+pose (tProd
+  (mkNamed "A")
+  (tSort
+     (Universe.of_levels
+        (inr
+           (Level.Level
+              "Sniper.aux_fun_tests.465"))))
+  (tApp
+    list_reif [tRel 0]))
+as blut0.
+pose (tProd
+  (mkNamed "A")
+  (tSort
+     (Universe.of_levels
+        (inr
+           (Level.Level
+              "Sniper.aux_fun_tests.387"))))
+  (tProd
+     {|
+       binder_name := nAnon;
+       binder_relevance := Relevant
+     |} (tRel 0)
+     (tProd
+        {|
+          binder_name := nAnon;
+          binder_relevance := Relevant
+        |}
+        (tApp
+           list_reif [tRel 1])
+        (tApp list_reif [tRel 2])))) as blut1.
+let list_info := fresh "list_info" in get_info_quote list list_info. 
+pose list_info.2 as list_indu. compute in list_indu. (* \Q pq ça ne calcule pas ? *)
+pose list_info.1.2 as list_I_app. compute in list_I_app.
+pose list_info.1.1.2 as list_lpars. compute in list_lpars.
+pose list_info.1.1.1.2 as list_total_args. compute in list_total_args.
+pose list_info.1.1.1.1.2 as list_list_args. compute in list_list_args.
+pose list_info.1.1.1.1.1.2 as list_list_ty. compute in list_list_ty.
+pose list_info.1.1.1.1.1.1.2 as list_ty_pars. compute in list_ty_pars.
+pose list_info.1.1.1.1.1.1.1 as list_npars.  hnf in list_npars. 
+(* Print list_I_app. *) (* gives the parameter i *)
+
+
+(* proj_one_constructor_default_var (i : term) (ty_default : term)
+ (I : inductive) (npars : nat) (nbproj : nat) (nbconstruct : nat)
+(ty_arg_constr : list (list term)) (return_type : term) *) 
+
+let x := proj_one_constructor_default_var  (tApp list_reif [tRel 0]) 
+ (tApp list_reif [tRel 0])  
+list 1 0 1 [t
+in pose x as y.
+
+Abort.
